repr without length

src/lowparse/LowParse.Repr.fst
@@ -50,50 +50,8 @@ let strong_parser_kind =
 
 let preorder (c:C.const_buffer LP.byte) = C.qbuf_pre (C.as_qbuf c)
 
-inline_for_extraction noextract
-let slice_of_const_buffer (b:C.const_buffer LP.byte) (len:uint_32{U32.v len <= C.length b})
-  : LP.slice (preorder b) (preorder b)
-  =
-    LP.({
-       base = C.cast b;
-       len = len
-    })
-
 let mut_p = LowStar.Buffer.trivial_preorder LP.byte
 
-
-/// A slice is a const uint_8* and a length.
-///
-/// It is a layer around LP.slice, effectively guaranteeing that no
-/// writes are performed via this pointer.
-///
-/// It allows us to uniformly represent `ptr t` backed by either
-/// mutable or immutable arrays.
-noeq
-type const_slice =
-  | MkSlice:
-      base:C.const_buffer LP.byte ->
-      slice_len:uint_32 {
-        UInt32.v slice_len <= C.length base//  /\
-        // slice_len <= LP.validator_max_length
-      } ->
-      const_slice
-
-let to_slice (x:const_slice)
-  : Tot (LP.slice (preorder x.base) (preorder x.base))
-  = slice_of_const_buffer x.base x.slice_len
-
-let of_slice (x:LP.slice mut_p mut_p {x.LP.len <= LP.validator_max_length} )
-  : Tot const_slice
-  = let b = C.of_buffer x.LP.base in
-    let len = x.LP.len in
-    MkSlice b len
-
-let live_slice (h:HS.mem) (c:const_slice) =
-    C.live h c.base
-
-let slice_as_seq (h:HS.mem) (c:const_slice) =
-    Seq.slice (C.as_seq h c.base) 0 (U32.v c.slice_len)
 
 (*** Pointer-based Representation types ***)
 
@@ -143,9 +101,7 @@ noeq
 type repr_ptr (t:Type) =
   | Ptr: b:C.const_buffer LP.byte ->
          meta:meta t ->
-         vv:t ->
-         length:U32.t { U32.v meta.len == C.length b /\
-                       meta.len == length /\
+         vv:t { U32.v meta.len == C.length b /\
                        vv == meta.v } ->
        repr_ptr t
 
@@ -155,10 +111,6 @@ let value #t (p:repr_ptr t) : GTot t = p.meta.v
 
 let repr_ptr_p (t:Type) (#k:strong_parser_kind) (parser:LP.parser k t) =
   p:repr_ptr t{ p.meta.parser_kind == k /\ p.meta.parser == parser }
-
-let slice_of_repr_ptr #t (p:repr_ptr t)
-  : GTot (LP.slice (preorder p.b) (preorder p.b))
-  = slice_of_const_buffer p.b p.meta.len
 
 let sub_ptr (p2:repr_ptr 'a) (p1: repr_ptr 'b) =
   exists pos len. Ptr?.b p2 `C.const_sub_buffer pos len` Ptr?.b p1
@@ -171,17 +123,6 @@ let intro_sub_ptr (x:repr_ptr 'a) (y:repr_ptr 'b) (from to:uint_32)
     (ensures
       x `sub_ptr` y)
   = ()
-
-/// TEMPORARY: DO NOT USE THIS FUNCTION UNLESS YOU REALLY HAVE SOME
-/// SPECIAL REASON FOR IT
-///
-/// It is meant to support migration towards an EverParse API that
-/// will eventually provide accessors and jumpers for pointers rather
-/// than slices
-inline_for_extraction noextract
-let temp_slice_of_repr_ptr #t (p:repr_ptr t)
-  : Tot (LP.slice (preorder p.b) (preorder p.b))
-  = slice_of_const_buffer p.b p.length
 
 (*** Validity ***)
 
@@ -201,15 +142,13 @@ let temp_slice_of_repr_ptr #t (p:repr_ptr t)
 ///
 ///    3. The bytes of the slice are indeed the representation of the
 ///       ghost value in wire format
-unfold
-let valid_slice (#t:Type) (#r #s:_) (slice:LP.slice r s) (meta:meta t) (h:HS.mem) =
-  LP.valid_content_pos meta.parser h slice 0ul meta.v meta.len /\
-  meta.repr_bytes == LP.bytes_of_slice_from_to h slice 0ul meta.len
 
 unfold
 let valid' (#t:Type) (p:repr_ptr t) (h:HS.mem) =
-  let slice = slice_of_const_buffer p.b p.meta.len in
-  valid_slice slice p.meta h
+  let meta = p.meta in
+  let b = C.cast p.b in
+  LP.bvalid_content_pos meta.parser h b 0ul meta.v meta.len /\
+  meta.repr_bytes == LP.bytes_of_buffer_from_to h b 0ul meta.len
 
 /// `valid`: abstract validity
 abstract
@@ -223,6 +162,16 @@ let reveal_valid ()
               {:pattern (valid #t p h)}
            valid #t p h <==> valid' #t p h)
   = ()
+
+let valid_repr_bytes
+  (#t:Type) (p:repr_ptr t) (h:HS.mem) (s: LP.serializer p.meta.parser)
+: Lemma
+  (requires (valid p h))
+  (ensures (
+    p.meta.repr_bytes == LP.serialize s p.meta.v
+  ))
+= LP.parse_serialize s p.meta.v;
+  LP.parse_injective p.meta.parser (LP.serialize s p.meta.v) p.meta.repr_bytes
 
 /// `fp r`: The memory footprint of a repr_ptr is the underlying pointer
 let fp #t (p:repr_ptr t)
@@ -246,52 +195,54 @@ let frame_valid #t (p:repr_ptr t) (l:B.loc) (h0 h1:HS.mem)
 
 (***  Contructors ***)
 /// `mk b from to p`:
-///    Constructing a `repr_ptr` from a sub-slice
+///    Constructing a `repr_ptr` from a const_buffer
 ///      b.[from, to)
 ///    known to be valid for a given wire-format parser `p`
 #set-options "--z3rlimit 20"
 inline_for_extraction noextract
-let mk_from_const_slice
+let mk_from_const_buffer
          (#k:strong_parser_kind) #t (#parser:LP.parser k t)
          (parser32:LS.parser32 parser)
-         (b:const_slice)
-         (from to:uint_32)
+         (b: C.const_buffer LP.byte)
+         (from:uint_32)
   : Stack (repr_ptr_p t parser)
     (requires fun h ->
-      LP.valid_pos parser h (to_slice b) from to)
+      LP.bvalid parser h (C.cast b) from)
     (ensures fun h0 p h1 ->
       B.(modifies loc_none h0 h1) /\
       valid p h1 /\
-      p.meta.v == LP.contents parser h1 (to_slice b) from /\
-      p.b `C.const_sub_buffer from (to - from)` b.base)
+      p.meta.v == LP.bcontents parser h1 (C.cast b) from /\
+      p.b `C.const_sub_buffer from p.meta.len` b)
   = let h = get () in
-    let slice = to_slice b in
-    LP.contents_exact_eq parser h slice from to;
+    let bb = C.cast b in
+    let to = Ghost.hide (LP.bget_valid_pos parser h bb from) in
+    LP.contents_exact_eq parser h (LP.slice_of_buffer bb) from (Ghost.reveal to);
     let meta :meta t = {
         parser_kind = _;
         parser = parser;
         parser32 = parser32;
-        v = LP.contents parser h slice from;
+        v = LP.bcontents parser h bb from;
         len = to - from;
-        repr_bytes = LP.bytes_of_slice_from_to h slice from to;
+        repr_bytes = LP.bytes_of_buffer_from_to h bb from to;
         meta_ok = ()
     } in
-    let sub_b = C.sub b.base from (to - from) in
+    let sub_b = C.sub b from (to - from) in
     let value =
       // Compute [.v]; this code will eventually disappear
-      let sub_b_bytes = FStar.Bytes.of_buffer (to - from) (C.cast sub_b) in
+      let to' : (to' : U32.t { to' == Ghost.reveal to }) = magic () in
+      let sub_b_bytes = FStar.Bytes.of_buffer (to' - from) (C.cast sub_b) in
       let Some (v, _) = parser32 sub_b_bytes in
       v
     in
-    let p = Ptr sub_b meta value (to - from) in
+    let p = Ptr sub_b meta value in
     let h1 = get () in
-    let slice' = slice_of_const_buffer sub_b (to - from) in
-    LP.valid_facts p.meta.parser h1 slice from; //elim valid_pos slice
-    LP.valid_facts p.meta.parser h1 slice' 0ul; //intro valid_pos slice'
+    let bb' = C.cast sub_b in
+    LP.bvalid_facts p.meta.parser h1 bb from; //elim valid_pos slice
+    LP.bvalid_facts p.meta.parser h1 bb' 0ul; //intro valid_pos slice'
     p
 
 /// `mk b from to p`:
-///    Constructing a `repr_ptr` from a LowParse slice
+///    Constructing a `repr_ptr` from a buffer
 ///      b.[from, to)
 ///    known to be valid for a given wire-format parser `p`
 inline_for_extraction
@@ -299,18 +250,18 @@ noextract
 let mk (#k:strong_parser_kind) #t (#parser:LP.parser k t)
        (parser32:LS.parser32 parser)
        #q
-       (slice:LP.slice (C.q_preorder q LP.byte) (C.q_preorder q LP.byte))
-       (from to:uint_32)
+       (b:B.mbuffer LP.byte (C.q_preorder q LP.byte) (C.q_preorder q LP.byte))
+       (from:uint_32)
   : Stack (repr_ptr_p t parser)
     (requires fun h ->
-      LP.valid_pos parser h slice from to)
+      LP.bvalid parser h b from)
     (ensures fun h0 p h1 ->
       B.(modifies loc_none h0 h1) /\
       valid p h1 /\
-      p.b `C.const_sub_buffer from (to - from)` (C.of_qbuf slice.LP.base) /\
-      p.meta.v == LP.contents parser h1 slice from)
-  = let c = MkSlice (C.of_qbuf slice.LP.base) slice.LP.len in
-    mk_from_const_slice parser32 c from to
+      p.b `C.const_sub_buffer from p.meta.len` (C.of_qbuf b) /\
+      p.meta.v == LP.bcontents parser h1 b from)
+  = let c = C.of_qbuf b in
+    mk_from_const_buffer parser32 c from
 
 /// A high-level constructor, taking a value instead of a slice.
 ///
@@ -339,6 +290,7 @@ let mk_from_serialize
          let size = size32 x in
          valid p h1 /\
          U32.v from + U32.v size <= U32.v b.LP.len /\
+         p.meta.len == size /\
          p.b == C.gsub (C.of_buffer b.LP.base) from size /\
          p.meta.v == x))
   = let size = size32 x in
@@ -347,12 +299,17 @@ let mk_from_serialize
     then None
     else begin
       let bytes = serializer32 x in
+      assert (size == FStar.Bytes.len bytes);
       let dst = B.sub b.LP.base from size in
       (if size > 0ul then FStar.Bytes.store_bytes bytes dst);
-        let to = from + size in
+      let to = from + size in
       let h = get () in
       LP.serialize_valid_exact serializer h b x from to;
-      let r = mk parser32 b from to in
+      LP.valid_bvalid_strong_prefix parser h b from;
+      LP.parse_serialize serializer x;
+      let r = mk parser32 b.LP.base from in
+      let h' = ST.get () in
+      valid_repr_bytes r h' serializer;
       Some r
     end
 
@@ -368,9 +325,7 @@ let length #t (p: repr_ptr t) (j:LP.jumper p.meta.parser)
     (ensures fun h n h' ->
       B.modifies B.loc_none h h' /\
       n == p.meta.len)
-  = let s = temp_slice_of_repr_ptr p in
-    (* TODO: Need to revise the type of jumpers to take a pointer as an argument, not a slice *)
-    j s 0ul
+  = j (C.cast p.b) 0ul
 
 /// `to_bytes`: for intermediate purposes only, extract bytes from the repr
 let to_bytes #t (p: repr_ptr t) (len:uint_32)
@@ -453,7 +408,7 @@ let valid_if_live_intro #t (r:repr_ptr t) (h:HS.mem)
             valid r h')
           [SMTPat (valid r h')]
         = let m = r.meta in
-          LP.valid_ext_intro m.parser h (slice_of_repr_ptr r) 0ul h' (slice_of_repr_ptr r) 0ul
+          LP.valid_ext_intro m.parser h (LP.slice_of_buffer (C.cast r.b)) 0ul h' (LP.slice_of_buffer (C.cast r.b)) 0ul
     in
     ()
 
@@ -510,7 +465,7 @@ let recall_stable_repr_ptr #t (r:stable_repr_ptr t)
           valid r h1)
         [SMTPat (valid r h)]
       = let m = r.meta in
-        LP.valid_ext_intro m.parser h (slice_of_repr_ptr r) 0ul h1 (slice_of_repr_ptr r) 0ul
+        LP.valid_ext_intro m.parser h (LP.slice_of_buffer (C.cast r.b)) 0ul h1 (LP.slice_of_buffer (C.cast r.b)) 0ul
      in
      let es =
        let m = r.meta in
@@ -576,15 +531,12 @@ let stash (rgn:ST.drgn) #t (r:repr_ptr t) (len:uint_32{len == r.meta.len})
      valid r' h1 /\
      r.meta == r'.meta)
  = let buf' = ralloc_and_blit rgn r.b len in
-   let s = MkSlice buf' len in
    let h = get () in
    let _ =
-     let slice = slice_of_const_buffer r.b len in
-     let slice' = slice_of_const_buffer buf' len in
-     LP.valid_facts r.meta.parser h slice 0ul; //elim valid_pos slice
-     LP.valid_facts r.meta.parser h slice' 0ul //intro valid_pos slice'
+     LP.bvalid_facts r.meta.parser h (C.cast r.b) 0ul; //elim valid_pos slice
+     LP.bvalid_facts r.meta.parser h (C.cast buf') 0ul //intro valid_pos slice'
    in
-   let p = Ptr buf' r.meta r.vv r.length in
+   let p = Ptr buf' r.meta r.vv in
    valid_if_live_intro p h;
    p
 
@@ -602,7 +554,7 @@ type field_accessor (#k1 #k2:strong_parser_kind)
      (#cl: LP.clens t1 t2) ->
      (#g: LP.gaccessor p1 p2 cl) ->
      (acc:LP.accessor g) ->
-     (jump:LP.jumper p2) ->
+//     (jump:LP.jumper p2) ->
      (p2': LS.parser32 p2) ->
      field_accessor p1 p2
 
@@ -616,10 +568,10 @@ let field_accessor_comp (#k1 #k2 #k3:strong_parser_kind)
                         (f23 : field_accessor p2 p3)
    : field_accessor p1 p3
    =
-   [@inline_let] let FieldAccessor acc12 j2 p2' = f12 in
-   [@inline_let] let FieldAccessor acc23 j3 p3' = f23 in
+   [@inline_let] let FieldAccessor acc12 (* j2 *) p2' = f12 in
+   [@inline_let] let FieldAccessor acc23 (* j3 *) p3' = f23 in
    [@inline_let] let acc13 = LP.accessor_compose acc12 acc23 () in
-     FieldAccessor acc13 j3 p3'
+     FieldAccessor acc13 (* j3 *) p3'
 
 unfold noextract
 let field_accessor_t
@@ -645,13 +597,12 @@ let get_field (#k1:strong_parser_kind) #t1 (#p1:LP.parser k1 t1)
               (f:field_accessor p1 p2)
    : field_accessor_t f
    = fun p ->
-     [@inline_let] let FieldAccessor acc jump p2' = f in
-     let b = temp_slice_of_repr_ptr p in
-     let pos = acc b 0ul in
-     let pos_to = jump b pos in
-     let q = mk p2' b pos pos_to in
+     [@inline_let] 
+     let FieldAccessor acc (*jump*) p2' = f in
+     let pos = acc (C.cast p.b) 0ul in
+     let q = mk p2' (C.cast p.b) pos in
      let h = get () in
-     assert (q.b `C.const_sub_buffer pos (pos_to - pos)` p.b);
+     assert (q.b `C.const_sub_buffer pos q.meta.len` p.b);
      assert (q `sub_ptr` p); //needed to trigger the sub_ptr_stable lemma
      assert (is_stable_in_region p ==> is_stable_in_region q);
      q
@@ -695,41 +646,38 @@ let read_field (#k1:strong_parser_kind) (#t1:_) (#p1:LP.parser k1 t1)
   = fun p ->
     [@inline_let]
     let FieldReader acc reader = f in
-    let b = temp_slice_of_repr_ptr p in
-    let pos = acc b 0ul in
-    reader b pos
+    let pos = acc (C.cast p.b) 0ul in
+    reader (C.cast p.b) pos
 
 (*** Positional representation types ***)
 
 /// `index b` is the type of valid indexes into `b`
-let index (b:const_slice)= i:uint_32{ i <= b.slice_len }
+let index (b: C.const_buffer LP.byte)= i:uint_32{ U32.v i <= C.length b }
 
 noeq
-type repr_pos (t:Type) (b:const_slice) =
+type repr_pos (t:Type) (b:C.const_buffer LP.byte) =
   | Pos: start_pos:index b ->
          meta:meta t ->
-         vv_pos:t -> //temporary
-         length:U32.t { U32.v start_pos + U32.v meta.len <= U32.v b.slice_len /\
-                        vv_pos == meta.v /\
-                        length == meta.len } ->
+         vv_pos:t //temporary
+                       { U32.v start_pos + U32.v meta.len <= C.length b /\
+                        vv_pos == meta.v  } ->
          repr_pos t b
 
 let value_pos #t #b (r:repr_pos t b) : GTot t = r.meta.v
 
 let as_ptr_spec #t #b (p:repr_pos t b)
   : GTot (repr_ptr t)
-  = Ptr (C.gsub b.base p.start_pos ((Pos?.meta p).len))
+  = Ptr (C.gsub b p.start_pos ((Pos?.meta p).len))
         (Pos?.meta p)
         (Pos?.vv_pos p)
-        (Pos?.length p)
 
 
 let const_buffer_of_repr_pos #t #b (r:repr_pos t b)
   : GTot (C.const_buffer LP.byte)
-  = C.gsub b.base r.start_pos r.meta.len
+  = C.gsub b r.start_pos r.meta.len
 
 /// `repr_pos_p`, the analog of `repr_ptr_p`
-let repr_pos_p (t:Type) (b:const_slice) #k (parser:LP.parser k t) =
+let repr_pos_p (t:Type) (b: C.const_buffer LP.byte) #k (parser:LP.parser k t) =
   r:repr_pos t b {
     r.meta.parser_kind == k /\
     r.meta.parser == parser
@@ -737,13 +685,13 @@ let repr_pos_p (t:Type) (b:const_slice) #k (parser:LP.parser k t) =
 
 (*** Validity ***)
 /// `valid`: abstract validity
-let valid_repr_pos (#t:Type) (#b:const_slice) (r:repr_pos t b) (h:HS.mem)
+let valid_repr_pos (#t:Type) (#b: C.const_buffer LP.byte) (r:repr_pos t b) (h:HS.mem)
   = valid (as_ptr_spec r) h /\
-    C.live h b.base
+    C.live h b
 
 /// `fp r`: The memory footprint of a repr_pos is the
 ///         sub-slice b.[from, to)
-let fp_pos #t (#b:const_slice) (r:repr_pos t b)
+let fp_pos #t (#b: C.const_buffer LP.byte) (r:repr_pos t b)
   : GTot B.loc
   = fp (as_ptr_spec r)
 
@@ -765,15 +713,14 @@ let frame_valid_repr_pos #t #b (r:repr_pos t b) (l:B.loc) (h0 h1:HS.mem)
 (*** Operations on repr_pos ***)
 
 /// End position
-/// On positional reprs, this is concretely computable
 let end_pos #t #b (r:repr_pos t b)
-  : index b
-  = r.start_pos + r.length
+  : GTot (index b)
+  = r.start_pos + r.meta.len
 
 abstract
 let valid_repr_pos_elim
   (#t: Type)
-  (#b: const_slice)
+  (#b: _)
   (r: repr_pos t b)
   (h: HS.mem)
 : Lemma
@@ -781,13 +728,12 @@ let valid_repr_pos_elim
     valid_repr_pos r h
   ))
   (ensures (
-    LP.valid_content_pos r.meta.parser h (to_slice b) r.start_pos r.meta.v (end_pos r)
+    LP.bvalid_content_pos r.meta.parser h (C.cast b) r.start_pos r.meta.v (end_pos r)
   ))
 = let p : repr_ptr t = as_ptr_spec r in
-  let slice = slice_of_const_buffer (Ptr?.b p) (Ptr?.meta p).len in
-  LP.valid_facts r.meta.parser h slice 0ul;
-  LP.valid_facts r.meta.parser h (to_slice b) r.start_pos;
-  LP.parse_strong_prefix r.meta.parser (LP.bytes_of_slice_from h slice 0ul) (LP.bytes_of_slice_from h (to_slice b) r.start_pos)
+  LP.bvalid_facts r.meta.parser h (C.cast (Ptr?.b p)) 0ul;
+  LP.bvalid_facts r.meta.parser h (C.cast b) r.start_pos;
+  LP.parse_strong_prefix r.meta.parser (LP.bytes_of_buffer_from h (C.cast (Ptr?.b p)) 0ul) (LP.bytes_of_buffer_from h (C.cast b) r.start_pos)
 
 /// Mostly just by inheriting operations on pointers
 let as_ptr #t #b (r:repr_pos t b)
@@ -797,20 +743,19 @@ let as_ptr #t #b (r:repr_pos t b)
     (ensures fun h0 ptr h1 ->
       ptr == as_ptr_spec r /\
       h0 == h1)
-  = let b = C.sub b.base r.start_pos (Ghost.hide r.meta.len) in
+  = let b = C.sub b r.start_pos (Ghost.hide r.meta.len) in
     let m = r.meta in
     let v = r.vv_pos in
-    let l = r.length in
-    Ptr b m v l
+    Ptr b m v
 
-let as_repr_pos #t (b:const_slice) (from to:index b) (p:repr_ptr t)
+let as_repr_pos #t (b: C.const_buffer LP.byte) (from:index b) (to: Ghost.erased (index b)) (p:repr_ptr t)
   : Pure (repr_pos t b)
     (requires
       from <= to /\
-      Ptr?.b p  == C.gsub b.base from (to - from))
+      Ptr?.b p  == C.gsub b from (to - from))
     (ensures fun r ->
       p == as_ptr_spec r)
-  = Pos from (Ptr?.meta p) (Ptr?.vv p) (to - from)
+  = Pos from (Ptr?.meta p) (Ptr?.vv p)
 
 /// `mk_repr_pos b from to p`:
 ///    Constructing a `repr_pos` from a sub-slice
@@ -819,39 +764,47 @@ let as_repr_pos #t (b:const_slice) (from to:index b) (p:repr_ptr t)
 inline_for_extraction
 let mk_repr_pos (#k:strong_parser_kind) #t (#parser:LP.parser k t)
                 (parser32:LS.parser32 parser)
-                (b:LP.slice mut_p mut_p{ LP.(b.len <= validator_max_length) })
-                (from to:index (of_slice b))
-  : Stack (repr_pos_p t (of_slice b) parser)
+                (b: B.mbuffer LP.byte mut_p mut_p)
+                (from:index (C.of_qbuf b))
+  : Stack (repr_pos_p t (C.of_qbuf b) parser)
     (requires fun h ->
-      LP.valid_pos parser h b from to)
+      LP.bvalid parser h b from)
     (ensures fun h0 r h1 ->
       B.(modifies loc_none h0 h1) /\
       valid_repr_pos r h1 /\
       r.start_pos = from /\
-      end_pos r = to /\
-      r.vv_pos == LP.contents parser h1 b from)
-  = as_repr_pos (of_slice b) from to (mk parser32 b from to)
+      r.vv_pos == LP.bcontents parser h1 b from)
+  = let h = ST.get () in
+    let to = Ghost.hide (LP.bget_valid_pos parser h b from) in
+    let r = mk parser32 b from in
+    LP.bvalid_facts parser h b from;
+    LP.parse_injective parser (LP.bytes_of_buffer_from h b from) ((Ptr?.meta r).repr_bytes);
+    as_repr_pos (C.of_qbuf b) from to r
 
 /// `mk b from to p`:
 ///    Constructing a `repr_pos` from a sub-slice
 ///      b.[from, to)
 ///    known to be valid for a given wire-format parser `p`
 inline_for_extraction
-let mk_repr_pos_from_const_slice
+let mk_repr_pos_from_const_buffer
          (#k:strong_parser_kind) #t (#parser:LP.parser k t)
          (parser32:LS.parser32 parser)
-         (b:const_slice)
-         (from to:index b)
+         (b: C.const_buffer LP.byte)
+         (from:index b)
   : Stack (repr_pos_p t b parser)
     (requires fun h ->
-      LP.valid_pos parser h (to_slice b) from to)
+      LP.bvalid parser h (C.cast b) from)
     (ensures fun h0 r h1 ->
       B.(modifies loc_none h0 h1) /\
       valid_repr_pos r h1 /\
       r.start_pos = from /\
-      end_pos r = to /\
-      r.vv_pos == LP.contents parser h1 (to_slice b) from)
-  = as_repr_pos b from to (mk_from_const_slice parser32 b from to)
+      r.vv_pos == LP.bcontents parser h1 (C.cast b) from)
+  = let h = ST.get () in
+    let to = Ghost.hide (LP.bget_valid_pos parser h (C.cast b) from) in
+    let r = mk_from_const_buffer  parser32 b from in
+    LP.bvalid_facts parser h (C.cast b) from;
+    LP.parse_injective parser (LP.bytes_of_buffer_from h (C.cast b) from) ((Ptr?.meta r).repr_bytes);
+    as_repr_pos b from to r
 
 /// A high-level constructor, taking a value instead of a slice.
 ///
@@ -865,9 +818,9 @@ let mk_repr_pos_from_serialize
   (parser32: LS.parser32 parser) (serializer32: LS.serializer32 serializer)
   (size32: LS.size32 serializer)
   (b:LP.slice mut_p mut_p{ LP.(b.len <= validator_max_length) })
-  (from:index (of_slice b))
+  (from: U32.t { from <= b.LP.len })
   (x: t)
-: Stack (option (repr_pos_p t (of_slice b) parser))
+: Stack (option (repr_pos_p t (C.of_qbuf b.LP.base) parser))
     (requires fun h ->
       LP.live_slice h b)
     (ensures fun h0 r h1 ->
@@ -875,7 +828,7 @@ let mk_repr_pos_from_serialize
       begin match r with
       | None ->
         (* not enough space in output slice *)
-        Seq.length (LP.serialize serializer x) > FStar.UInt32.v (b.LP.len - from)
+        Seq.length (LP.serialize serializer x) > U32.v b.LP.len - FStar.UInt32.v from
       | Some r ->
         valid_repr_pos r h1 /\
         r.start_pos == from /\
@@ -886,11 +839,11 @@ let mk_repr_pos_from_serialize
 = let size = size32 x in
   match (mk_from_serialize parser32 serializer32 size32 b from x) with
   | None -> None
-  | Some p -> Some (as_repr_pos (of_slice b) from (from + size) p)
+  | Some p -> Some (as_repr_pos (C.of_qbuf b.LP.base) from (from + size) p)
 
 /// Accessors on positional reprs
 unfold
-let field_accessor_pos_post (#b:const_slice) (#t1:Type) (p:repr_pos t1 b)
+let field_accessor_pos_post (#b:C.const_buffer LP.byte) (#t1:Type) (p:repr_pos t1 b)
                             (#k2: strong_parser_kind)
                             (#t2:Type)
                             (#p2: LP.parser k2 t2)
@@ -906,7 +859,7 @@ unfold
 let get_field_pos_t (#k1: strong_parser_kind) (#t1: Type) (#p1: LP.parser k1 t1)
                     (#k2: strong_parser_kind) (#t2: Type) (#p2: LP.parser k2 t2)
                     (f:field_accessor p1 p2)
-   = (#b:const_slice) ->
+   = (#b: _) ->
      (pp:repr_pos_p t1 b p1) ->
     Stack (repr_pos_p t2 b p2)
      (requires fun h ->
@@ -923,20 +876,17 @@ let get_field_pos (#k1: strong_parser_kind) (#t1: Type) (#p1: LP.parser k1 t1)
                   (f:field_accessor p1 p2)
  : get_field_pos_t f
  = fun #b pp ->
-    [@inline_let] let FieldAccessor acc jump p2' = f in
-    let p = as_ptr pp in
-    let bb = temp_slice_of_repr_ptr p in
-    let pos = acc bb 0ul in
-    let pos_to = jump bb pos in
-    let q = mk p2' bb pos pos_to in
-    let len = pos_to - pos in
-    assert (Ptr?.b q `C.const_sub_buffer pos len` Ptr?.b p);
-    as_repr_pos b (pp.start_pos + pos) (pp.start_pos + pos + len) q
+    [@inline_let]
+    let FieldAccessor acc (*jump*) p2' = f in
+    let h = ST.get () in
+    valid_repr_pos_elim pp h;
+    let pos = acc (C.cast b) pp.start_pos in
+    mk_repr_pos_from_const_buffer p2' b pos
 
 unfold
 let read_field_pos_t (#k1: strong_parser_kind) (#t1: Type) (#p1: LP.parser k1 t1)
                      #t2 (f:field_reader p1 t2)
-  = (#b:const_slice) ->
+  = (#b:_) ->
     (p:repr_pos_p t1 b p1) ->
     Stack t2
     (requires fun h ->
